shallow/LLVM_Shallow_RS.thy
@@ -697,15 +697,15 @@ lemma (in llvm_prim_arith_setup) llvm_from_bool_inline[llvm_inline]:
 
 subsubsection \<open>Products\<close>
   
-lemma inline_prod_case[llvm_inline]: "(\<lambda>(a,b). f a b) = (\<lambda>x. doM { a\<leftarrow>ll_extract_fst x; b \<leftarrow> ll_extract_snd x; f a b })"  
-  by (auto simp: ll_extract_fst_def ll_extract_snd_def)
+lemma inline_prod_case[llvm_inline]: "(\<lambda>(a,b). f a b) = (\<lambda>x. doM { a\<leftarrow>prod_extract_fst x; b \<leftarrow> prod_extract_snd x; f a b })"  
+  by (auto simp: prod_ops_simp)
   
 lemma inline_return_prod_case[llvm_inline]: 
   "return (case x of (a,b) \<Rightarrow> f a b) = (case x of (a,b) \<Rightarrow> return (f a b))" by (rule prod.case_distrib)
   
   
-lemma inline_return_prod[llvm_inline]: "return (a,b) = doM { x \<leftarrow> ll_insert_fst init a; x \<leftarrow> ll_insert_snd x b; return x }"  
-  by (auto simp: ll_insert_fst_def ll_insert_snd_def)
+lemma inline_return_prod[llvm_inline]: "return (a,b) = doM { x \<leftarrow> prod_insert_fst init a; x \<leftarrow> prod_insert_snd x b; return x }"  
+  by (auto simp: prod_ops_simp)
   
 subsubsection \<open>Marking of constants\<close>    
 definition "ll_const x \<equiv> return x"
